Trestle/Solver/IncCNF.lean
@@ -9,6 +9,18 @@ import Trestle.Solver.Dimacs
 
 namespace Trestle.Solver.Dimacs
 
+def parseCube (maxVar : Nat) (s : String) : Except String ICube := do
+  if s.startsWith "a " then
+    parseClause maxVar <| s.drop 2
+  else
+    .error s!"expected cube, but does not start with `a `: {s}"
+
+def parseCubes (maxVar : Nat) (s : String) : Except String (List ICube) :=
+  s.splitOn "\n"
+  |>.map (·.trim)
+  |>.filter (!·.isEmpty)
+  |>.mapM (parseCube maxVar)
+
 def printCubes [Monad m] (print : String → m Unit) (cubes : List IClause) : m Unit := do
   for cube in cubes do
     print <| "a " ++ formatClause cube ++ "\n"
